Add ObserveStrictValid and ObserveTypePtr
Replace tptsto_valid_ptr with tptsto_type_ptr and instances for deduction of consequences.

theories/lang/cpp/logic/pred.v
@@ -206,10 +206,6 @@ Module Type CPP_LOGIC (Import CC : CPP_LOGIC_CLASS)
       Observe2 [| v1 = v2 |] (@tptsto σ t q1 p v1) (@tptsto σ t q2 p v2).
     Global Existing Instance tptsto_agree.
 
-    Axiom tptsto_valid_ptr : forall σ t q p v,
-      Observe (strict_valid_ptr p) (@tptsto σ t q p v).
-    Global Existing Instance tptsto_valid_ptr.
-
     Axiom tptsto_nonvoid : forall {σ} ty (q : Qp) p v,
       Observe [| ty <> Tvoid |] (@tptsto σ ty q p v).
     Global Existing Instance tptsto_nonvoid.
@@ -412,6 +408,11 @@ Module Type CPP_LOGIC (Import CC : CPP_LOGIC_CLASS)
       type_ptr (resolve := σ) ty p |--
       Exists align, [| @align_of σ ty = Some align |] ** aligned_ptr align p.
 
+    (* Intentionally not an instance, and exposed through
+    [tptsto_observe_type_ptr]. *)
+    Axiom tptsto_type_ptr : forall (σ : genv) ty q p v,
+      Observe (type_ptr ty p) (tptsto ty q p v).
+
     (**
     Recall that [type_ptr] and [strict_valid_ptr] don't include
     past-the-end pointers... *)
@@ -495,8 +496,46 @@ Module Type VALID_PTR_AXIOMS.
 End VALID_PTR_AXIOMS.
 Declare Module Export VALID_PTR : VALID_PTR_AXIOMS.
 
+Class ObserveStrictValid `{Σ : cpp_logic} P p := {
+  obs_strict_valid :> Observe (strict_valid_ptr p) P;
+  obs_rel_valid :> Observe (relaxed_valid_ptr p) P
+}.
+Hint Mode ObserveStrictValid ! ! ! - : typeclass_instances.
+
+Class ObserveTypePtr `{Σ : cpp_logic} P p (σ : genv) ty := {
+  type_ptr__strict_valid :> ObserveStrictValid P p;
+  obs_type_ptr :> Observe (type_ptr ty p) P;
+}.
+Hint Mode ObserveTypePtr ! ! ! - - - : typeclass_instances.
+
 Section with_cpp.
   Context `{Σ : cpp_logic}.
+
+  Lemma observe_strict_valid_intro
+    `{Hobs : !Observe (strict_valid_ptr p) P} :
+    ObserveStrictValid P p.
+  Proof.
+    split => //.
+    by rewrite /Observe Hobs strict_valid_relaxed.
+  Qed.
+
+  Lemma observe_type_ptr_intro (σ : genv)
+    `{Hobs : !Observe (type_ptr ty p) P} :
+    ObserveTypePtr P p σ ty.
+  Proof.
+    split => //.
+    apply: observe_strict_valid_intro.
+    by rewrite /Observe Hobs type_ptr_strict_valid.
+  Qed.
+
+  Global Instance tptsto_observe_type_ptr (σ : genv) ty q p v :
+    ObserveTypePtr (tptsto ty q p v) p σ ty.
+  Proof. apply observe_type_ptr_intro, tptsto_type_ptr. Qed.
+
+  Local Instance tptsto_strict_valid_ptr (σ : genv) ty q p v :
+    Observe (strict_valid_ptr p) (tptsto ty q p v) := _.
+  Local Instance tptsto_valid_ptr : forall σ t q p v,
+    Observe (valid_ptr p) (tptsto (σ := σ) t q p v) := _.
 
   Lemma valid_ptr_sub {σ : genv} p ty i vt :
     0 <= i -> _valid_ptr vt (p .., o_sub σ ty i) |-- _valid_ptr vt p.
@@ -643,6 +682,7 @@ Section with_cpp.
     iApply (pinned_ptr_aligned_divide with "P A").
   Qed.
 
+  (* Just wrappers. *)
   Lemma valid_ptr_nullptr : |-- valid_ptr nullptr.
   Proof. exact: _valid_ptr_nullptr. Qed.
   Lemma strict_valid_ptr_nullptr : |-- strict_valid_ptr nullptr.
